Logic/FirstOrder/Arith/StrictHierarchy.lean
@@ -1,0 +1,134 @@
+import Logic.FirstOrder.Arith.Hierarchy
+
+namespace LO
+
+namespace FirstOrder
+
+variable {L : Language} [L.LT] {μ : Type v}
+
+namespace Arith
+
+inductive StrictHierarchy : Polarity → ℕ → {n : ℕ} → Semiformula L μ n → Prop
+  | zero {Γ p}                                : DeltaZero p → StrictHierarchy Γ s p
+  | sigma {s n} {p : Semiformula L μ (n + 1)} : StrictHierarchy Π s p → StrictHierarchy Σ (s + 1) (∃' p)
+  | pi {s n} {p : Semiformula L μ (n + 1)}    : StrictHierarchy Σ s p → StrictHierarchy Π (s + 1) (∀' p)
+  | ex {s n} {p : Semiformula L μ (n + 1)}    : StrictHierarchy Σ (s + 1) p → StrictHierarchy Σ (s + 1) (∃' p)
+  | all {s n} {p : Semiformula L μ (n + 1)}   : StrictHierarchy Π (s + 1) p → StrictHierarchy Π (s + 1) (∀' p)
+
+lemma DeltaZero.of_open {p : Semiformula L μ n} : p.Open → DeltaZero p := Hierarchy.of_open
+
+namespace StrictHierarchy
+
+lemma rew {p : Semiformula L μ₁ n₁} (h : StrictHierarchy Γ s p) (ω : Rew L μ₁ n₁ μ₂ n₂) :
+    StrictHierarchy Γ s (ω.hom p) := by
+  induction h generalizing μ₂ n₂ <;> try simp
+  case zero h => exact zero <| (Hierarchy.rew_iff (ω := ω)).mpr h
+  case sigma ih => exact (ih ω.q).sigma
+  case pi ih => exact (ih ω.q).pi
+  case ex ih => exact (ih ω.q).ex
+  case all ih => exact (ih ω.q).all
+
+lemma succ {Γ} {p : Semiformula L μ₁ n₁} (h : StrictHierarchy Γ s p) :
+    StrictHierarchy Γ (s + 1) p := by
+  induction h
+  case zero h => exact zero h
+  case sigma ih => exact ih.sigma
+  case pi ih => exact ih.pi
+  case ex ih => exact ih.ex
+  case all ih => exact ih.all
+
+lemma zero_iff_delta_zero {Γ} {p : Semiformula L μ n} :
+    StrictHierarchy Γ 0 p ↔ DeltaZero p := by
+  constructor
+  · rintro ⟨h⟩; exact h
+  · intro h; exact zero h
+
+end StrictHierarchy
+
+def SHClass (L : Language) [L.LT] (Γ : Polarity) (s : ℕ) : Class L where
+  domain := StrictHierarchy Γ s
+  rewrite_closed := by intro p hp f; exact hp.rew _
+
+notation Γ "ᴴ("s")" => SHClass _ Γ s
+
+abbrev SHClassIn (Γ s) (T : Theory L) := (SHClass L Γ s).eqvClosure T
+
+notation Γ "ᴴ("s")[" T "]" => SHClassIn Γ s T
+
+abbrev DeltaZeroIn (T : Theory L) := (SHClass L Σ 0).eqvClosure T
+
+notation "Δ₀[" T "]" => DeltaZeroIn T
+
+lemma SHClassIn.eqDeltaZero (T : Theory L) (Γ) : Γᴴ(0)[T] = Δ₀[T] := by
+  simp [SHClassIn, DeltaZeroIn]; congr 1
+  ext p; simp [SHClass, Set.mem_def, StrictHierarchy.zero_iff_delta_zero]
+
+namespace SHClassIn
+
+variable (Γ : Polarity) (s : ℕ) (T : Theory L)
+
+open StrictHierarchy Semiformula
+
+lemma accumlative_succ (Γ Γ' s) : Γᴴ(s)[T] ≤ Γ'ᴴ(s + 1)[T] := by
+  rintro p ⟨p', hp', Hp⟩
+  cases Γ <;> cases Γ'
+  · exact ⟨p', hp'.succ, Hp⟩
+  · exact ⟨∀' Rew.bShift.hom p', (rew hp' _).pi, Equivalent.trans (Equivalent.dummy_quantifier_all p') Hp⟩
+  · exact ⟨∃' Rew.bShift.hom p', (rew hp' _).sigma, Equivalent.trans (Equivalent.dummy_quantifier_ex p') Hp⟩
+  · exact ⟨p', hp'.succ, Hp⟩
+
+lemma accumlative (Γ Γ') {s s'} (h : s < s') : Γᴴ(s)[T] ≤ Γ'ᴴ(s')[T] := by
+  generalize hk : s' - s - 1 = k
+  have : s' = s + 1 + k := by simp [←hk, Nat.sub_sub]; exact (Nat.sub_eq_iff_eq_add' h).mp rfl
+  rcases this with rfl
+  clear h hk
+  induction' k with k ih
+  · simp; exact accumlative_succ T Γ Γ' s
+  · simp [show s + 1 + k.succ = s + 1 + k + 1 from by simp [Nat.add_succ]]
+    exact Class.LE.trans ih (accumlative_succ T _ _ _)
+
+@[simp] lemma delta_zero_le : Δ₀[T] ≤ Γᴴ(s)[T] := by
+  cases s
+  · simp [SHClassIn.eqDeltaZero]; rfl
+  · rw [←SHClassIn.eqDeltaZero T Γ]; exact accumlative T Γ Γ (by simp)
+
+lemma openClass_le : openClass L ≤ SHClass L Σ 0 := by
+  intro p hp
+  simp [SHClass, Set.mem_def, zero_iff_delta_zero]
+  exact Hierarchy.of_open hp
+
+lemma openClass_le' : openClass L ≤ Γᴴ(s)[T] :=
+  Class.LE.trans openClass_le (Class.LE.trans (Class.le_eqvClosure _ _) (delta_zero_le Γ s T))
+
+instance atom : (Γᴴ(s)[T]).Atom := Class.of_le (openClass L) _ (openClass_le' Γ s T)
+
+end SHClassIn
+
+namespace DeltaZeroIn
+
+variable (Γ : Polarity) (s : ℕ) (T : Theory L)
+
+open Hierarchy SHClassIn StrictHierarchy Semiformula
+
+instance atom : (Δ₀[T]).Atom := SHClassIn.atom Σ 0 T
+
+instance not : (Δ₀[T]).Not := ⟨by
+  rintro p ⟨p', hp', Hp⟩
+  exact ⟨~p',
+    zero_iff_delta_zero.mpr
+      (by simp [←Hierarchy.zero_iff_delta_zero (Γ := Σ), pi_zero_iff_sigma_zero]; exact zero_iff_delta_zero.mp hp'),
+    Hp.not⟩⟩
+
+instance and : (Δ₀[T]).And := ⟨by
+  rintro p q ⟨p', hp', Hp⟩ ⟨q', hq', Hq⟩
+  have hp' : DeltaZero p' := zero_iff_delta_zero.mp hp'
+  have hq' : DeltaZero q' := zero_iff_delta_zero.mp hq'
+  exact ⟨p' ⋏ q', zero_iff_delta_zero.mpr (Hierarchy.and hp' hq'), Hp.and Hq⟩⟩
+
+instance or : (Δ₀[T]).Or := ⟨by
+  rintro p q ⟨p', hp', Hp⟩ ⟨q', hq', Hq⟩
+  have hp' : DeltaZero p' := zero_iff_delta_zero.mp hp'
+  have hq' : DeltaZero q' := zero_iff_delta_zero.mp hq'
+  exact ⟨p' ⋎ q', zero_iff_delta_zero.mpr (Hierarchy.or hp' hq'), Hp.or Hq⟩⟩
+
+end DeltaZeroIn
